最抽象的一集

题目：

You are given an integer array `nums` sorted in **non-decreasing** order.

Build and return _an integer array_ `result` _with the same length as_ `nums` _such that_ `result[i]` _is equal to the **summation of absolute differences** between_ `nums[i]` _and all the other elements in the array._

In other words, `result[i]` is equal to `sum(|nums[i]-nums[j]|)` where `0 <= j < nums.length` and `j != i` (**0-indexed**).

**Example 1:**

**Input:** nums = `[2,3,5]`
**Output:** `[4,3,5]`
**Explanation:** Assuming the arrays are 0-indexed, then
`result[0] = |2-2| + |2-3| + |2-5| = 0 + 1 + 3 = 4,`
`result[1] = |3-2| + |3-3| + |3-5| = 1 + 0 + 2 = 3,`
`result[2] = |5-2| + |5-3| + |5-5| = 3 + 2 + 0 = 5.`

**Example 2:**

**Input:** nums = `[1,4,6,8,10]`
**Output:** `[24,15,13,15,21]`

**Constraints:**

- `2 <= nums.length <= 105`
- `1 <= nums[i] <= nums[i + 1] <= 104`

use `5` as an example here:
`|5-2| + |5-3| + |5-5|`
is basically
`5*3 - (2+3+5)`
as 5 >= all the elements in the array.

And for `2`:
`|2-2| + |2-3| + |2-5|` = `(2+3+5) - 2*3`
as 2 <= all the elements in the array

拿到的数组是按照大小排序的。

所以我们可以把整个数组分割成两个，在i=x的循环中，x之前的数一定都小于他，反之在它之后的都大于它，于是我们可以用x的index位置的个数+1的x减去所有在x之前的数的sum。另一边则是反过来的，从数组末尾加起来的数的sum减去x的index位置的个数（由于我们已经在上一步骤减去一次x自己位置的数，这里x的数量不需要+1）
`((nums[i]*(i+1)) - prefixSum[i]) + (suffixSum[i+1] - nums[i] * (n-i-1))`
`// n here is the length of nums`
但是这样的设计会让导致我们需要考虑 i+1 超出数组边界的情况，观察这个式子的性质，我们可以挪动一部分元素：
`((nums[i]*i) - prefixSum[i]) + (suffixSum[i] - (nums[i] * (n-i-1)));`
对比`suffixSum[i]`和`suffixSum[i+1]`，可以发现其实他们的区别就是`nums[i]`本身。所以我们可以通过将最前面的一个`nums[i]`移动到`suffixSum`那边来减少麻烦。

---

草稿：

```

[2,3,5]

prefixsum and suffixsum array:

pre:

prefixsum[0] = nums[0]

prefixsum[i] = prefixSum[i - 1] + nums[i];

[2,5,10]

suffixsum:

suffixsum[n-1] = nums[n-1]

suffixsum[n - i - 1] = suffixsum[n - i] + nums[n - i - 1];

[10,8,5]


result:
[0+1+3=4,1+0+2=3,3+2+0+5]

((nums[i] * i) - prefixSum[i]) + (suffixSum[i] - (nums[i] * (n - i - 1)));
(2*0 - 2) + (10 - 2*2) = 4 

= ((nums[i]*(i+1)) - prefixSum[i]) + (suffixSum[i+1] - nums[i] * (n-i))

```